Work on translating syntax of STLC to both Coq and Top in a relational way

Language/Reflect.v
@@ -2,52 +2,39 @@
 Inductive Ty : Type :=
   | TDiscrete : Set -> Ty
   | Tunit : Ty
-  | Tpair : Ty -> Ty -> Ty.
+  | Tpair : Ty -> Ty -> Ty
+  | Tfunc : Ty -> Ty -> Ty.
 
-Inductive Expr : Ty -> Type :=
-| Ett : Expr Tunit
-| Econst : forall {A : Set}, A -> Expr (TDiscrete A)
-| Efst : forall {A B}, Expr (Tpair A B) -> Expr A
-| Esnd : forall {A B}, Expr (Tpair A B) -> Expr B
-| Epair : forall {A B}, Expr A -> Expr B -> Expr (Tpair A B).
+Require Import Coq.Lists.List. 
+Import ListNotations.
+
+Fixpoint prodTy (xs : list Ty) : Ty := match xs with
+ | nil => Tunit
+ | x :: xs' => Tpair (prodTy xs') x
+ end.
 
 Fixpoint dcoqT (t : Ty) : Type := match t with
 | Tunit => unit
 | TDiscrete A => A
 | Tpair a b => prod (dcoqT a) (dcoqT b)
+| Tfunc a b => dcoqT a -> dcoqT b
 end.
 
-Fixpoint dcoq {A} (e : Expr A) : dcoqT A := match e with
-| Ett => tt
-| Econst x => x
-| Efst e' => fst (dcoq e')
-| Esnd e' => snd (dcoq e')
-| Epair a b => pair (dcoq a) (dcoq b)
-end.
-
-Fixpoint dcoq_eq {A : Ty} : dcoqT A -> dcoqT A -> Prop
-  := match A with
-| Tunit => fun _ _ => True
-| TDiscrete _ => eq
-| Tpair a b => fun e1 e2 => dcoq_eq (fst e1) (fst e2) /\ dcoq_eq (snd e1) (snd e2)
-end.
-
-Theorem dcoq_eq_eq {A : Ty} : forall (x y : dcoqT A),
-  dcoq_eq x y -> x = y.
-Proof.
-intros. induction A.
-- assumption.
-- destruct x, y. reflexivity.
-- destruct x, y, H. f_equal; auto.
-Qed.
+Definition dcoqTG Γ A := dcoqT (prodTy Γ) -> dcoqT A.
 
 Section Cont.
 Require Import Spec.Category Spec.Discrete.
 Import Category.
 Import Discrete.
+Require Import Spec.CCC.CCC.
+Import CCC.
 Context {U : Type} {ccat : CCat U} {cmc : CMC U}
+  {ccc : CCCOps U}
   {D : Type -> U} {power : Type -> U -> U} 
-  {Dops : DiscreteOps D power}.
+  {Dops : DiscreteOps D power}
+  {cmcprops : CMC_Props U}
+  {cccprops : CCCProps U}
+  {discrete_props : DiscreteProps D power}.
 
 Local Open Scope obj.
 Local Open Scope morph.
@@ -55,89 +42,408 @@ Local Open Scope morph.
 Fixpoint dcontT (t : Ty) : U := match t with
 | TDiscrete A => D A
 | Tunit => unit
-| Tpair a b => (dcontT a * dcontT b)%obj
+| Tpair a b => dcontT a * dcontT b
+| Tfunc a b => dcontT a ==> dcontT b
 end.
 
-Fixpoint dcont {A} (e : Expr A) : unit ~~> dcontT A 
-  := match e with
-  | Ett => tt
-  | Econst x => discrete_pt _ _ x
-  | Efst e' => fst ∘ dcont e'
-  | Esnd e' => snd ∘ dcont e'
-  | Epair a b => pair (dcont a) (dcont b)
-  end.
+Definition dcontTG Γ A := dcontT (prodTy Γ) ~~> dcontT A.
 
-Fixpoint d_discrete_ok {t} : Expr t -> Prop := match t with
-| TDiscrete A => fun e => dcont e == discrete_pt _ _ (dcoq e )
-| Tunit => fun _ => True
-| Tpair a b => fun e => d_discrete_ok (Efst e)
-   /\ d_discrete_ok (Esnd e)
+Fixpoint Rel {ty : Ty} : dcoqT ty -> unit ~~> dcontT ty -> Prop := match ty with
+| TDiscrete A => fun e1 e2 => e2 == discrete_pt _ _ e1
+| Tunit => fun _ _ => True
+| Tpair _ _ => fun e1 e2 => Rel (Datatypes.fst e1) (fst ∘ e2)
+    /\ Rel (Datatypes.snd e1) (snd ∘ e2)
+| Tfunc _ _ => fun f1 f2 => forall x1 x2, Rel x1 x2 ->
+    Rel (f1 x1) (eval ∘ ⟨ f2 , x2 ⟩) 
 end.
 
-Context {cmcprops : CMC_Props U (ccat := ccat) (cmc := cmc)}.
-Context {discrete_props : DiscreteProps D power}.
-
-Lemma d_discrete_ok_respectful {t} : forall (e1 e2 : Expr t),
-  dcoq e1 = dcoq e2 -> 
-  dcont e1 == dcont e2 -> d_discrete_ok e1 -> d_discrete_ok e2.
+Lemma Rel_uniq_cont {ty : Ty} : forall (eC : dcoqT ty)
+  (e1 e2 : unit ~~> dcontT ty),
+  Rel eC e1 -> Rel eC e2 -> e1 == e2.
 Proof.
-induction t; simpl; intros.
-- rewrite <- H, <- H0. assumption.
+induction ty; simpl; intros.
+- rewrite H, H0. reflexivity. 
+- rewrite (unit_uniq e1), (unit_uniq e2).
+  reflexivity.
+- destruct H, H0. 
+  rewrite (pair_uniq e1), (pair_uniq e2).
+  apply pair_Proper. eapply IHty1; eassumption.
+  eapply IHty2; eassumption.
+- rewrite <- (abstract_eval e1), <- (abstract_eval e2).
+  unfold parallel.
+Abort.
+
+Fixpoint dcoq_eq {A : Ty} : dcoqT A -> dcoqT A -> Prop
+  := match A as A' return dcoqT A' -> dcoqT A' -> Prop with
+| Tunit => fun _ _ => True
+| TDiscrete _ => Logic.eq
+| Tpair a b => fun e1 e2 => dcoq_eq (Datatypes.fst e1) (Datatypes.fst e2)
+    /\ dcoq_eq (Datatypes.snd e1) (Datatypes.snd e2)
+| Tfunc a b => fun f1 f2 => forall x1 x2 : dcoqT a, dcoq_eq x1 x2 -> dcoq_eq (f1 x1) (f2 x2)
+end.
+
+Definition dcoqG_eq {Γ A} : dcoqTG Γ A -> dcoqTG Γ A -> Prop :=
+  fun f1 f2 => forall x1 x2, dcoq_eq x1 x2 -> dcoq_eq (f1 x1) (f2 x2).
+
+Require Import Morphisms.
+Instance dcoq_eq_Equiv {A} : Equivalence (@dcoq_eq A).
+Proof.
+constructor; unfold Reflexive, Symmetric, Transitive.
+- induction A; intros; simpl; auto.
+  intros. 
+Admitted.
+
+Instance dcoqG_eq_Equiv {Γ A} : Equivalence (@dcoqG_eq Γ A).
+Proof.
+constructor; unfold Reflexive, Symmetric, Transitive, dcoqG_eq; intros.
+- admit.
+- symmetry. apply H. symmetry. assumption.
+- etransitivity. apply H. eassumption. apply H0. reflexivity.
+Admitted. 
+
+Lemma Rel_respectful {ty} :
+  Proper (dcoq_eq ==> eq ==> Basics.impl) (@Rel ty).
+Proof.
+unfold Proper, respectful, Basics.impl.
+induction ty; simpl; intros.
+- subst. rewrite <- H1. symmetry. assumption.
 - auto.
-- destruct H1. split.
-  + eapply IHt1. 3: eassumption. simpl.
-    f_equal. assumption. simpl.
-    apply compose_Proper. reflexivity. assumption.
-  + eapply IHt2. 3: eassumption. simpl.
-    f_equal. assumption. simpl.
-    apply compose_Proper. reflexivity. assumption.
+- destruct H, H1. split.
+  + eapply IHty1. eassumption.
+    apply compose_Proper. reflexivity. eassumption. assumption.
+  + eapply IHty2. eassumption.
+    apply compose_Proper. reflexivity. eassumption. assumption.
+- eapply IHty2. apply H. Focus 2. rewrite <- H0. reflexivity. reflexivity.
+  apply H1. eassumption.
 Qed.
 
-Lemma d_discrete_ok_holds {t} (e : Expr t) : d_discrete_ok e.
+Instance Rel_respectful' {ty}
+  : Proper (dcoq_eq ==> eq ==> iff) (@Rel ty).
 Proof.
-induction e; simpl.
-- auto. 
-- reflexivity. 
-- simpl in IHe. destruct IHe. assumption.
-- simpl in IHe. destruct IHe. assumption.
-- split. apply (d_discrete_ok_respectful e1).
-  simpl. reflexivity. simpl. rewrite pair_fst. reflexivity.
-  assumption.
-  apply (d_discrete_ok_respectful e2).
-  simpl. reflexivity. simpl. rewrite pair_snd.
-  reflexivity. assumption.
+unfold Proper, respectful. intros.
+split; apply Rel_respectful; repeat (assumption || symmetry).
 Qed.
 
-Theorem full_abstract : forall (A : Ty) (e1 e2 : Expr A),
-  dcoq_eq (dcoq e1) (dcoq e2) -> dcont e1 == dcont e2.
+Definition subst_coq {Γ A B} (e : dcoqTG (A :: Γ) B)
+  (x : dcoqTG Γ A) : dcoqTG Γ B
+  := fun ctxt => e (ctxt, x ctxt).
+
+Definition subst_cont {Γ A B} (e : dcontTG (A :: Γ) B)
+  (x : dcontTG Γ A) : dcontTG Γ B
+  := e ∘ ⟨ id , x ⟩.
+
+Fixpoint RelG {Γ} {A : Ty} : dcoqTG Γ A -> dcontTG Γ A -> Prop := 
+  match Γ as Γ' return dcoqTG Γ' A -> dcontTG Γ' A -> Prop with
+| [] => fun e1 e2 => Rel (e1 Datatypes.tt) e2
+| X :: Xs => fun f1 f2 => forall x1 x2, RelG x1 x2 ->
+     RelG (subst_coq f1 x1) (subst_cont f2 x2)
+end.
+
+Lemma RelG_respectful {Γ A}
+  : Proper (dcoqG_eq ==> eq ==> Basics.impl) (@RelG Γ A).
 Proof.
-intros. induction A.
-- pose proof (d_discrete_ok_holds e1).
-  unfold d_discrete_ok in H0. rewrite H0; clear H0.
-  pose proof (d_discrete_ok_holds e2).
-  unfold d_discrete_ok in H0. rewrite H0. 
-  rewrite H. reflexivity.
-- rewrite (unit_uniq (dcont e1)).
-  rewrite (unit_uniq (dcont e2)). reflexivity.
-- destruct H. 
-  rewrite pair_uniq. rewrite (pair_uniq (dcont e2)). 
-  apply pair_Proper.
-  specialize (IHA1 (Efst e1) (Efst e2) H).
-  simpl in IHA1. assumption.
-  specialize (IHA2 (Esnd e1) (Esnd e2) H0).
-  simpl in IHA2. assumption.
+unfold Proper, respectful. 
+induction Γ; unfold dcoqG_eq, Basics.impl; simpl; intros.
+- rewrite <- H, <- H0. eassumption. auto.
+- unfold Basics.impl in IHΓ. eapply IHΓ. 3: apply H1. 3: eassumption. 
+  unfold dcoqG_eq. intros. 
+  apply H. simpl. split. assumption.
+  assert (dcoqG_eq x1 x1) as H4 by reflexivity.
+  apply H4. assumption.
+  unfold subst_cont. rewrite H0. reflexivity.
 Qed.
 
-Definition test : nat :=
- Datatypes.snd ( 3 , 4 ).
-
-Definition test_Expr : Expr (TDiscrete nat) :=
-  Esnd (Epair (Econst 3) (Econst 4)).
-
-Theorem test_ok : dcoq (test_Expr) = test.
+Instance RelG_respectful' {Γ A}
+  : Proper (dcoqG_eq ==> eq ==> iff) (@RelG Γ A).
 Proof.
+unfold Proper, respectful. intros.
+split; apply RelG_respectful; repeat (assumption || symmetry).
+Qed.
+
+
+
+
+
+
+
+Inductive Constant {Γ} {A : Ty} : Type := MkConst
+  { Ccoq : dcoqTG Γ A
+  ; Ccont : dcontTG Γ A
+  ; Crel : RelG Ccoq Ccont }.
+
+Arguments Constant : clear implicits.
+
+Definition Constant_subst {Γ A B} (f : Constant (A :: Γ) B)
+  (x : Constant Γ A) : Constant Γ B.
+Proof.
+destruct f, x; simpl in *.
+unshelve econstructor.
+- eapply subst_coq; eassumption. 
+- eapply subst_cont; eassumption.
+- apply Crel0. assumption. 
+Defined.
+
+Definition Constant_swap {Γ A B C} (x : Constant (A :: B :: Γ) C)
+  : Constant (B :: A :: Γ) C.
+Proof.
+unshelve econstructor.
+- unfold dcoqTG in *. simpl in *.
+  intros. apply (Ccoq x). destruct X as ((g & a) & b).
+  simpl. auto. 
+- unfold dcontTG in *. simpl in *.
+  refine (Ccont x ∘ _).
+  apply (⟨ ⟨ fst ∘ fst , snd ⟩ , snd ∘ fst ⟩).
+- apply undefined.
+Defined.
+
+Definition Constant_weak {Γ A B} (x : Constant Γ B)
+  : Constant (A :: Γ) B.
+Proof.
+unshelve econstructor.
+- unfold dcoqTG in *. simpl. intros.
+  apply (Ccoq x). apply (Datatypes.fst X).
+- unfold dcontTG in *. simpl. 
+  apply (Ccont x ∘ fst).
+- simpl. intros. unfold subst_coq, subst_cont.
+  simpl. rewrite <- compose_assoc. rewrite pair_fst.
+  rewrite compose_id_right. apply x.
+Defined.
+
+Inductive member {A} : A -> list A -> Type :=
+  | member_here : forall {x xs}, member x (x :: xs)
+  | member_there : forall {x y ys}, member x ys -> member x (y :: ys).
+
+Inductive termDB {G : list Ty} : Ty -> Type :=
+  | VarDB : forall {t}, member t G -> termDB t
+  | ConstDB : forall {A : Ty}, Constant G A -> termDB A
+  | AbsDB : forall {dom ran}, @termDB (dom :: G) ran -> termDB (Tfunc dom ran)
+  | AppDB : forall {dom ran}, termDB (Tfunc dom ran) -> termDB dom -> termDB ran.
+
+Arguments termDB : clear implicits.
+
+Ltac inv H := inversion H; clear H; subst.
+
+Definition swap_member {X : Type} {A B C : X} {Γ : list X}
+  (x : member C (A :: B :: Γ))
+  : member C (B :: A :: Γ).
+Proof.
+inv x. apply member_there. apply member_here.
+inv X0. apply member_here. apply member_there. apply member_there.
+assumption.
+Defined.
+
+Fixpoint swapDB {Γ A B C} (e : termDB (A :: B :: Γ) C)
+  : termDB (B :: A :: Γ) C
+  := match e with
+ | VarDB m => VarDB (swap_member m)
+ | ConstDB c => ConstDB (Constant_swap c)
+ | AbsDB f => undefined _
+ | AppDB f x => AppDB (swapDB f) (swapDB x)
+end.
+
+Lemma member_rect1 :
+forall (A : Type) (P : forall (a : A) (b : A) (l : list A), member a (b :: l) -> Type),
+(forall (x : A) (xs : list A), P x x xs member_here) ->
+(forall (x y b : A) (ys : list A) (m : member x (b :: ys)),
+ P x b ys m -> P x y (b :: ys) (member_there m)) ->
+forall (y : A) (b : A) (l : list A) (m : member y (b :: l)), P y b l m.
+Proof.
+intros A P X X0.
+pose (fun l : list A => match l as ll return forall (a : A), member a ll -> Type with
+ | [] => fun a mem => False
+ | x :: xs => fun a => P a x xs
+ end) as P'.
+assert (forall l a mem, P' l a mem).
+intros.
+induction mem. 
+- simpl. auto.
+- simpl. destruct ys. simpl in *. contradiction. 
+  apply X0.  simpl in IHmem. assumption.
+- intros. apply (X1 (b :: l) y m).
+Defined.
+
+Lemma termDB_rect1 :
+forall P : forall (A : Ty) (G : list Ty) (t : Ty), termDB (A :: G) t -> Type,
+(forall A (G : list Ty) (t : Ty) (m : member t (A :: G)), P A G t (VarDB m)) ->
+(forall A' (G : list Ty) (A : Ty) (c : Constant (A' :: G) A), P A' G A (ConstDB c)) ->
+(forall A (G : list Ty) (dom ran : Ty) (t : termDB (A :: dom :: G) ran),
+ P A (dom :: G) ran t -> P dom G (Tfunc A ran) (AbsDB t)) ->
+(forall A (G : list Ty) (dom ran : Ty) (t : termDB (A :: G) (Tfunc dom ran)),
+ P A G (Tfunc dom ran) t -> forall t0 : termDB (A :: G) dom, P A G dom t0 -> P A G ran (AppDB t t0)) ->
+forall A (G : list Ty) (t : Ty) (t0 : termDB (A :: G) t), P A G t t0.
+Proof.
+intros P X X0 X1 X2.
+pose (fun G : list Ty => match G as GG return forall t : Ty, termDB GG t -> Type with
+ | [] => fun t term => True
+ | A :: G' => P A G'
+ end) as P'.
+assert (forall G t t0, P' G t t0).
+intros. 
+induction t0; destruct G; simpl; auto.
+intros A G. specialize (X3 (A :: G)). assumption.
+Defined.
+
+Definition substDB1_xx :
+  forall A Γ B, termDB (A :: Γ) B -> Constant Γ A -> termDB Γ B.
+Proof.
+apply (termDB_rect1 (fun A Γ B _ => Constant Γ A -> termDB Γ B));
+  intros.
+- generalize dependent X. generalize dependent G.
+  generalize dependent A. generalize dependent t.
+  apply (member_rect1 _ (fun t A G _ => Constant G A -> termDB G t)). 
+  + intros. apply ConstDB. assumption.
+  + intros. apply VarDB. assumption.
+- apply ConstDB. eapply Constant_subst; eassumption.
+- apply AbsDB. admit. 
+- eapply AppDB. apply X. assumption. apply X0. assumption.
+Admitted. 
+
+Fixpoint substDB {Γ A B} (e : termDB (A :: Γ) B)
+  : Constant Γ A -> termDB Γ B :=
+ match e with
+ | VarDB m => match m with
+   | member_here => fun k => ConstDB k
+   | member_there next => fun _ => VarDB next
+   end
+ | ConstDB c => fun k => ConstDB (Constant_subst c k)
+ | AbsDB f => undefined _
+ | AppDB f x => fun k => AppDB (substDB f k) (substDB x k)
+end.
+
+
+Lemma lookup {G : list Ty} {t : Ty} (m : member t G)
+  (e : dcoqT (prodTy G)) : dcoqT t.
+Proof.
+induction m; simpl in *; intros.
+- exact (Datatypes.snd e).
+- exact (IHm (Datatypes.fst e)).
+Defined.
+
+Axiom undefined : forall A, A.
+
+Set Asymmetric Patterns.
+
+Fixpoint dcoq_DB {Γ : list Ty} {A : Ty} (e : termDB Γ A)
+ : dcoqT (prodTy Γ) -> dcoqT A
+  := match e with
+| VarDB _ m => fun ctxt => lookup m ctxt
+| ConstDB _ (MkConst c _ _) => fun ctxt => c ctxt
+| AbsDB _ _ lam => fun ctxt x => dcoq_DB lam (ctxt , x)
+| AppDB _ _ f x => fun ctxt => (dcoq_DB f ctxt) (dcoq_DB x ctxt)
+end.
+
+Lemma substDB_coq  {Γ A B} (e : termDB (A :: Γ) B) (C : Constant Γ A)
+  : dcoqG_eq (subst_coq (dcoq_DB e) (Ccoq C))
+             (dcoq_DB (substDB e C)).
+Proof.
+generalize dependent C.
+generalize dependent B. generalize dependent Γ.
+generalize dependent A. 
+apply (termDB_rect1 (fun A Γ B e => 
+  forall C, dcoqG_eq (subst_coq (dcoq_DB e) (Ccoq C)) (dcoq_DB (substDB e C)))); intros.
+- unfold subst_coq. admit.
+- simpl. destruct c, C. simpl.
+  unfold subst_coq. reflexivity.
+Admitted.
+
+Definition dcoq_closed {A : Ty} (e : termDB [] A)
+  : dcoqT A := dcoq_DB e Datatypes.tt.
+
+
+Lemma lookup_cont (G : list Ty) (t : Ty) (m : member t G)
+  : dcontT (prodTy G) ~~> dcontT t.
+Proof.
+induction m; intros.
+- exact (snd).
+- exact (IHm ∘ fst).
+Defined.
+
+Definition dcont_DB {Γ : list Ty} {A : Ty} (e : termDB Γ A)
+  : dcontT (prodTy Γ) ~~> dcontT A.
+Proof.
+induction e.
+- apply lookup_cont. assumption.
+- induction c. assumption.
+- simpl. apply abstract. apply IHe.
+- refine (eval ∘ _). eapply pair; eassumption.
+Defined.
+
+Lemma substDB_cont  {Γ A B} (e : termDB (A :: Γ) B) (C : Constant Γ A)
+  : subst_cont (dcont_DB e) (Ccont C) == 
+             dcont_DB (substDB e C).
+Proof.
+Admitted.
+
+
+Lemma pair_parallel_snd : forall {A B C} (f : A ~~> B)
+  (x : A ~~> C), ⟨ f , x ⟩ == (f ⊗ id) ∘ ⟨ id , x ⟩.
+Proof.
+intros. rewrite parallel_pair. rewrite compose_id_right, compose_id_left.
 reflexivity.
 Qed.
+
+Theorem fst_constant {Γ A B} : Constant Γ (Tfunc (Tpair A B) A).
+Proof.
+unshelve econstructor; simpl.
+- unfold dcoqTG. simpl. intros. destruct X0. assumption.
+- unfold dcontTG. simpl.
+  apply abstract. apply (fst ∘ snd).
+- induction Γ; simpl; intros.
+  + destruct x1, H. simpl in *. rewrite pair_parallel_snd. 
+    rewrite compose_assoc. rewrite eval_abstract.
+    rewrite <- compose_assoc. rewrite pair_snd. assumption.
+  + eapply RelG_respectful'. 3 :eassumption. reflexivity.
+    unfold subst_cont.
+    unfold dcontTG in *. 
+    pose proof (abstract_ext (B := dcontT A) (fst (B := dcontT B) ∘ snd) ⟨ id, x2 ⟩).
+    rewrite H0. apply abstract_Proper.
+    rewrite <- compose_assoc. rewrite parallel_snd.
+    rewrite compose_id_left. reflexivity.
+Defined.
+
+Lemma RelG_substDB {Γ A B} (e : termDB (A :: Γ) B)
+  (C : Constant Γ A) :
+  RelG (dcoq_DB e) (dcont_DB e) ->
+  RelG (dcoq_DB (substDB e C)) (dcont_DB (substDB e C)).
+Proof.
+generalize dependent C.
+Admitted.
+
+  
+Theorem compiler_correct : forall Γ A (e : termDB Γ A),
+  RelG (dcoq_DB e) (dcont_DB e).
+Proof.
+intros. induction e.
+- induction m.
+  + simpl. intros. unfold subst_coq, subst_cont. simpl. 
+    rewrite pair_snd. assumption. 
+  + simpl in *. intros. eapply RelG_respectful'. 3: apply IHm.
+    reflexivity. unfold subst_cont.
+    rewrite <- compose_assoc. simpl. rewrite pair_fst.
+    rewrite compose_id_right. reflexivity.
+- induction c. assumption.
+- simpl. induction G; simpl in *; intros.
+  + eapply Rel_respectful'. simpl. 3: apply IHe. Unshelve.
+    Focus 4. unfold dcoqTG. simpl. intros; assumption.
+    unfold subst_coq. reflexivity.
+    rewrite pair_parallel_snd. rewrite compose_assoc.
+    rewrite eval_abstract. apply compose_Proper. reflexivity.
+    Focus 3. unfold dcontTG. simpl. assumption. reflexivity.
+    simpl. assumption.
+  + eapply RelG_respectful'. 3: apply IHG. Unshelve. 
+    Focus 4.
+    eapply substDB. Focus 2. eapply Constant_weak.
+    econstructor; eassumption. apply swapDB. assumption.
+    admit. admit. admit.
+- induction G; intros.
+  + simpl. eapply IHe1. assumption.
+  + repeat intro. pose (MkConst _ _ x1 x2 H) as C.
+    change x1 with (Ccoq C). change x2 with (Ccont C).
+    eapply RelG_respectful'.
+    apply substDB_coq. apply substDB_cont.
+    simpl. apply IHG; apply RelG_substDB; assumption.
+Admitted.
+
 
 Class IsProb {Prob : Type -> Type} :=
   { Ret : forall {A}, Prob A
